Split variables into three types (node, message, general)

tlc/assert/variable.v
@@ -1,28 +1,50 @@
 From mathcomp.ssreflect
 Require Import ssreflect eqtype ssrbool ssrnat seq path.
+From tlc.utility
+Require Import seq.
+
+Require Export message_variable node_variable general_variable.
 
 Set Implicit Arguments.
 Unset Strict Implicit.
 Unset Printing Implicit Defensive.
 
 Inductive variable : Type :=
-| V : nat -> variable.
+| Vnode : node_variable -> variable
+| Vmessage : message_variable -> variable
+| Vgeneral : general_variable -> variable.
 
 (* Equality *)
 Section variable_eq.
 
   Definition eq_variable (x x' : variable) :=
     match x, x' with
-    | V n, V n' => n == n'
+    | Vnode nx, Vnode nx' => nx == nx'
+    | Vnode _, _ => false
+    | Vmessage mx, Vmessage mx' => mx == mx'
+    | Vmessage _, _ => false
+    | Vgeneral gx, Vgeneral gx' => gx == gx'
+    | Vgeneral _, _ => false
     end.
 
   Lemma eq_variableP : Equality.axiom eq_variable.
   Proof.
-    case=> n; case=> n'; rewrite /eq_variable /=; try by constructor.
-    - (* V *)
-      case Hn: (n == n');
-        [move/eqP: Hn => ?; subst n' | constructor];
-        last by case=> ?; subst n'; rewrite eqxx in Hn.
+    case=> [nx | mx | gx]; case=> [nx' | mx' | gx'];
+      rewrite /eq_variable /=; try by constructor.
+    - (* Vnode *)
+      case Hnx: (nx == nx');
+        [move/eqP: Hnx => ?; subst nx' | constructor];
+        last by case=> ?; subst nx'; rewrite eqxx in Hnx.
+      by constructor.
+    - (* Vmessage *)
+      case Hmx: (mx == mx');
+        [move/eqP: Hmx => ?; subst mx' | constructor];
+        last by case=> ?; subst mx'; rewrite eqxx in Hmx.
+      by constructor.
+    - (* Vgeneral *)
+      case Hgx: (gx == gx');
+        [move/eqP: Hgx => ?; subst gx' | constructor];
+        last by case=> ?; subst gx'; rewrite eqxx in Hgx.
       by constructor.
   Qed.
 
@@ -33,35 +55,33 @@ Section variable_eq.
 
 End variable_eq.
 
-(* Flexible variables *)
-Notation Vfn := (V 0).
-Notation Vfd := (V 1).
-Notation Vfo := (V 2).
-Notation Vfe := (V 3).
-Notation Vfors := (V 4).
-Notation Vfois := (V 5).
-Notation Vfs := (V 6).
-Notation Vfs' := (V 7).
-
-(* Rigid variables *)
-Notation Vrn := (V 8).
-Notation Vrd := (V 9).
-Notation Vro := (V 10).
-Notation Vre := (V 11).
-Notation Vrors := (V 12).
-Notation Vrois := (V 13).
-Notation Vrs := (V 14).
-Notation Vri := (V 15).
+(* Coercions *)
+Coercion Vnode : node_variable >-> variable.
+Coercion Vmessage : message_variable >-> variable.
+Coercion Vgeneral : general_variable >-> variable.
 
 (* Arbitrary variables *)
-Definition first_var := V 16.
-Definition unwrap_var x := match x with V n => n end.
-Definition next_var x := V (S (unwrap_var x)).
+Definition next_var x :=
+  match x with
+  | Vnode nx => Vnode (next_node_var nx)
+  | Vmessage mx => Vmessage (next_message_var mx)
+  | Vgeneral gx => Vgeneral (next_general_var gx)
+  end.
 Definition fresh_var x xs :=
-  let: ns := map unwrap_var xs in
-  let: ns' := sort (fun a b => a < b) (undup ns) in
-  let: xs' := map V ns' in
-  if x \in xs' then last first_var xs' else x.
+  match x with
+  | Vnode nx =>
+    let nxs := osomes [seq
+      if x is Vnode nx then Some nx else None | x <- xs] in
+    Vnode (fresh_node_var nx nxs)
+  | Vmessage mx =>
+    let mxs := osomes [seq
+      if x is Vmessage mx then Some mx else None | x <- xs] in
+    Vmessage (fresh_message_var mx mxs)
+  | Vgeneral gx =>
+    let gxs := osomes [seq
+      if x is Vgeneral gx then Some gx else None | x <- xs] in
+    Vgeneral (fresh_general_var gx gxs)
+  end.
 Lemma fresh_var_unique x xs : ~(fresh_var x xs \in xs).
 Proof.
   (* TODO *)
