tlc/assert/message_variable.v
@@ -1,0 +1,51 @@
+From mathcomp.ssreflect
+Require Import ssreflect eqtype ssrbool ssrnat seq path.
+
+Set Implicit Arguments.
+Unset Strict Implicit.
+Unset Printing Implicit Defensive.
+
+Inductive message_variable : Type :=
+| MV : nat -> message_variable.
+
+(* Equality *)
+Section message_variable_eq.
+
+  Definition eq_message_variable (x x' : message_variable) :=
+    match x, x' with
+    | MV n, MV n' => n == n'
+    end.
+
+  Lemma eq_message_variableP : Equality.axiom eq_message_variable.
+  Proof.
+    case=> n; case=> n'; rewrite /eq_message_variable /=; try by constructor.
+    - (* V *)
+      case Hn: (n == n');
+        [move/eqP: Hn => ?; subst n' | constructor];
+        last by case=> ?; subst n'; rewrite eqxx in Hn.
+      by constructor.
+  Qed.
+
+  Canonical message_variable_eqMixin :=
+    Eval hnf in EqMixin eq_message_variableP.
+  Canonical message_variable_eqType :=
+    Eval hnf in EqType message_variable message_variable_eqMixin.
+
+End message_variable_eq.
+
+(* Rigid variables *)
+Notation Vrm := (MV 0).
+
+(* Arbitrary variables *)
+Definition first_message_var := MV 1.
+Definition unwrap_message_var x := match x with MV n => n end.
+Definition next_message_var x := MV (S (unwrap_message_var x)).
+Definition fresh_message_var x xs :=
+  let: ns := map unwrap_message_var xs in
+  let: ns' := sort (fun a b => a < b) (undup ns) in
+  let: xs' := map MV ns' in
+  if x \in xs' then last first_message_var xs' else x.
+Lemma fresh_message_var_unique x xs : ~(fresh_message_var x xs \in xs).
+Proof.
+  (* TODO *)
+Admitted.
